pulse/ulib/experimental/Steel.PCM.Memory.fsti
@@ -318,6 +318,36 @@ val gather_action
 val alloc_action (#a:Type u#1) (#pcm:pcm a) (e:inames) (x:a{compatible pcm x x})
   : action_except (ref a pcm) e emp (fun r -> pts_to r x)
 
+let property (a:Type)
+  = a -> prop
+
+val witnessed (#a:Type u#1)
+              (#pcm:pcm a)
+              (r:ref a pcm)
+              (fact:property a)
+  : prop
+
+let stable_property (#a:Type) (pcm:pcm a)
+  = fact:property a {
+       FStar.Preorder.stable fact (Steel.PCM.Preorder.preorder_of_pcm pcm)
+    }
+
+val witness (#a:Type) (#pcm:pcm a)
+            (e:inames)
+            (r:ref a pcm)
+            (fact:stable_property pcm)
+            (v:Ghost.erased a)
+            (_:squash (forall z. compatible pcm v z ==> fact z))
+  : action_except unit e (pts_to r v) (fun _ -> pts_to r v `star` pure (witnessed r fact))
+
+val recall (#a:Type u#1) (#pcm:pcm a) (#fact:property a)
+           (e:inames)
+           (r:ref a pcm)
+           (v:Ghost.erased a)
+  : action_except (v1:Ghost.erased a{compatible pcm v v1}) e
+                  (pts_to r v `star` pure (witnessed r fact))
+                  (fun v1 -> pts_to r v `star` pure (fact v1))
+
 (**** Invariants *)
 
 (**
